switched to new version of the setup using "ordered expressions", which are Proper functions from a context to an output type; defined the monad of downward-closed sets; started defining the trace monad

theories/Monad.v
@@ -1,139 +1,59 @@
 Require Export SepTypes.OrderedType.
-Require Export SepTypes.DownSet.
+Require Export SepTypes.OExpr.
 
 
 (***
- *** Monads over Ordered Types
+ *** The monad typeclass
  ***)
 
-Class MonadOps (M: forall A `{OType A}, Type) : Type :=
-  {
-    returnM : forall {A} `{OType A}, A -> M A;
+Class MonadOps M `{OTypeF M} : Type :=
+  { returnM : forall {A} `{OType A}, A -o> M A _;
     bindM : forall {A B} `{OType A} `{OType B},
-        M A -> (A -> M B) -> M B;
-  }.
+        M A _ -o> (A -o> M B _) -o> M B _ }.
 
-Class Monad (M: forall A `{OType A}, Type) `{OTypeF M} `{MonadOps M} : Prop :=
+Definition oreturn {ctx} `{MonadOps} {A} `{OType A} : OExpr ctx (A -o> M A _) :=
+  const_ofun returnM.
+Definition obind {ctx} `{MonadOps} {A B} `{OType A} `{OType B} :
+  OExpr ctx (M A _ -o> (A -o> M B _) -o> M B _) :=
+  const_ofun bindM.
+Notation "'do' x <- m1 ; m2" :=
+  (obind @o@ m1 @o@ mkLam (fun x => m2)) (at level 60, right associativity).
+
+
+Class Monad M `{MonadOps M} : Prop :=
   {
-    (* Proper-ness requirements *)
-    Proper_returnM {A} `{OType A} :>
-      Proper (oleq ==> oleq) (returnM (M:=M) (A:=A));
-    Proper_bindM {A B} `{OType A} `{OType B} :>
-      Proper (oleq ==> oleq ==> oleq) (bindM (M:=M) (A:=A) (B:=B));
+    monad_return_bind :
+      forall {ctx A B} `{OType A} `{OType B} (f: OExpr ctx (A -o> M B _)) x,
+        obind @o@ (oreturn @o@ x) @o@ f =o= f @o@ x;
 
-    (* Standard monad laws, which require bind functions to be Proper *)
-    monad_return_bind {A B} `{OType A} `{OType B} a (f : A -> M B) :
-      Proper (oleq ==> oleq) f ->
-      bindM (returnM a) f =o= f a;
-    monad_bind_return {A} `{OType A} (m : M A) :
-      bindM m returnM =o= m;
-    monad_assoc {A B C} `{OType A} `{OType B} `{OType C}
-                m (f: A -> M B) (g: B -> M C) :
-      Proper (oleq ==> oleq) f ->
-      Proper (oleq ==> oleq) g ->
-      bindM (bindM m f) g =o= bindM m (fun x => bindM (f x) g);
-  }.
+    monad_bind_return :
+      forall {ctx A} `{OType A} (m: OExpr ctx (M A _)),
+        obind @o@ m @o@ oreturn =o= m;
 
-
-Class MonadStateOps St `{OType St} (M: forall A `{OType A}, Type) : Type :=
-  { getM : M St;
-    putM : St -> M unit;
-  }.
-
-Class MonadState St `{OType St} (M: forall A `{OType A}, Type) `{OTypeF M}
-      `{MonadOps M} `{MonadStateOps St M} : Prop :=
-  {
-    monad_state_monad :> Monad M;
-
-    Proper_putM :> Proper (oleq ==> oleq) putM;
-
-    monad_state_get :
-      forall A `{OType A} (m : M A),
-        bindM getM (fun _ => m) =o= m;
-
-    monad_state_get_put :
-      forall A `{OType A} (f : St -> unit -> M A),
-        bindM getM (fun s => bindM (putM s) (f s))
-        =o= bindM getM (fun s => f s tt);
-
-    monad_state_put_get :
-      forall A `{OType A} s (f : unit -> St -> M A),
-        bindM (putM s) (fun u => bindM getM (f u))
-        =o= bindM (putM s) (fun u => f u s);
-
-    monad_state_put_put :
-      forall A `{OType A} s1 s2 (f : unit -> unit -> M A),
-        bindM (putM s1) (fun u => bindM (putM s2) (f u))
-        =o= bindM (putM s2) (f tt)
-  }.
-
-
-Class MonadFixOps (M: forall A `{OType A}, Type) : Type :=
-  {
-    fixM : forall {A B} `{OType A} `{OType B},
-      ((A -> M B) -> (A -> M B)) -> A -> M B;
-  }.
-
-Class MonadFix (M: forall A `{OType A}, Type)
-      `{OTypeF M} `{MonadFixOps M} : Prop :=
-  {
-    Proper_fixM {A B} `{OType A} `{OType B} :>
-      Proper (oleq ==> oleq) (fixM (M:=M) (A:=A) (B:=B));
-    fixM_correct :
-      forall {A B} `{OType A} `{OType B} (f: (A -> M B) -> (A -> M B)),
-        Proper (oleq ==> oleq) f ->
-        fixM f =o= f (fixM f)
-  }.
-
-Class MonadErrorOps (M: forall A `{OType A}, Type) : Type :=
-  {
-    errorM : forall {A} `{OType A}, M A;
-  }.
-
-Class MonadError (M: forall A `{OType A}, Type)
-      `{OTypeF M} `{MonadOps M} `{MonadErrorOps M} : Prop :=
-  {
-    bindM_errorM :
-      forall {A B} `{OType A} `{OType B} (f: A -> M B),
-        bindM errorM f =o= errorM;
+    monad_assoc :
+      forall {ctx A B C} `{OType A} `{OType B} `{OType C}
+             m (f: OExpr ctx (A -o> M B _)) (g: OExpr ctx (B -o> M C _)),
+        obind @o@ (obind @o@ m @o@ f) @o@ g
+        =o=
+        obind @o@ m @o@ (ofun x => obind @o@ (ovar f @o@ ovar x) @o@ ovar g);
   }.
 
 
 (***
- *** The Fixed-Point Monad
+ *** The Identity Monad
  ***)
 
-Definition FixM A `{OType A} := DownSet A.
+Definition Identity A `{OType A} := A.
 
-Instance OTypeF_FixM : OTypeF FixM := OType_DownSet.
+Instance OTypeF_Identity : OTypeF Identity :=
+  fun _ ot => ot.
 
-Instance MonadOps_FixM : MonadOps FixM :=
-  { returnM := fun _ _ => downClose;
-    bindM := fun _ _ _ _ => bindDownSet }.
+Instance IdMonad_MonadOps : MonadOps Identity :=
+  { returnM := fun A _ => oexpr (ofun x => x);
+    bindM := fun A B _ _ =>
+               oexpr (ofun m => ofun (f : A -o> B ) => ovar f @o@ ovar m) }.
 
-Instance Monad_FixM : Monad FixM.
+Instance IdMonad : Monad Identity.
 Proof.
-  constructor.
-  - apply Proper_downClose.
-  - apply Proper_bindDownSet.
-  - intros; apply DownSet_return_bind; assumption.
-  - intros; apply DownSet_bind_return; assumption.
-  - intros; apply DownSet_assoc.
+  constructor; intros; apply funOExt; intros; simpl; reflexivity.
 Qed.
-
-Instance MonadFixOps_FixM : MonadFixOps FixM :=
-  { fixM := fun _ _ _ _ => fixDownSet }.
-
-Instance MonadFix_FixM : MonadFix FixM.
-Proof.
-  constructor.
-  - intros. admit. (* FIXME: prove this, or fix the property *)
-  - intros. apply fixDownSetUnfold. assumption.
-Admitted.
-
-
-(***
- *** The Fixed-Point State Monad
- ***)
-
-(* FIXME... *)
