theories/MonadFix.v
@@ -1,0 +1,117 @@
+Require Export SepTypes.Monad.
+
+(***
+ *** Monads with Fixed-points
+ ***)
+
+Class MonadFixOps M `{OTypeF M} : Type :=
+  { fixM : forall {A B} `{OType A} `{OType B},
+      ((A -o> M B _) -o> (A -o> M B _)) -o> (A -o> M B _); }.
+
+Definition ofix {ctx} `{MonadFixOps} {A B} `{OType A} `{OType B} :
+  OExpr ctx (((A -o> M B _) -o> (A -o> M B _)) -o> (A -o> M B _)) :=
+  const_ofun fixM.
+
+
+Class MonadFix M {OF:OTypeF M} `{@MonadOps M OF} `{@MonadFixOps M OF} : Prop :=
+  { Monad_MonadFix :> Monad M;
+    FixedPoint_ofix :
+      forall {ctx A B} `{OType A} `{OType B}
+             (f: OExpr ctx ((A -o> M B _) -o> (A -o> M B _))),
+        ofix @o@ f =o= f @o@ (ofix @o@ f)
+  }.
+
+Class MonadBottomOps M `{OTypeF M} : Type :=
+  { bottomM : forall {A} `{OType A}, M A _ }.
+
+Definition obottom {ctx} `{MonadBottomOps} {A} `{OType A} : OExpr ctx (M A _) :=
+  const_ofun bottomM.
+
+Class MonadBottom M {OF:OTypeF M} `{@MonadOps M OF}
+      `{@MonadBottomOps M OF} : Prop :=
+  { Monad_MonadBottom :> Monad M;
+    Bottom_MonadBottom : forall {ctx A} `{OType A} (m: OExpr ctx (M A _)),
+        obottom <o= m }.
+
+
+(***
+ *** The Fixed-point Monad = Downwards-closed sets
+ ***)
+
+(* The type of downward-closed sets *)
+Definition DownSet A `{OType A} := Flip A -o> Prop.
+
+Instance OTypeF_DownSet : OTypeF DownSet := fun _ _ => _.
+
+(* The Monad operations for downward-closed sets *)
+Instance MonadOps_DownSet : MonadOps DownSet :=
+  {| returnM :=
+       fun A _ =>
+         oexpr (ofun (x:A) => ofun (y:Flip A) => oappr @o@ ovar y @o@ ovar x);
+     bindM :=
+       fun A B _ _ =>
+         oexpr (ofun m => ofun f => ofun (y:Flip B) =>
+                oexists2 @o@ (ofun x => ovar f @o@ ovar x @o@ ovar y) @o@ ovar m)
+  |}.
+
+Lemma flipLeftAdj {A} `{OType A} (x: A) (y: Flip A) :
+  flip x <o= y <-> unflip y <o= x.
+Proof.
+  destruct y; simpl; reflexivity.
+Qed.
+
+Lemma flipRightAdj {A} `{OType A} (x: Flip A) (y: A) :
+  x <o= flip y <-> y <o= unflip x.
+Proof.
+  destruct x; simpl; reflexivity.
+Qed.
+
+Lemma flipAdjEq {A} `{OType A} (x: A) (y: Flip A) :
+  flip x =o= y <-> x =o= unflip y.
+Proof.
+  destruct y; simpl. split; intro e; destruct e; split; assumption.
+Qed.
+
+Instance Monad_DownSet : Monad DownSet.
+Proof.
+  constructor; intros; apply funOExt; intro celem; apply funOExt.
+  { intro y; simpl; split.
+    - intros [ z pf1 pf2 ]. rewrite <- pf2. assumption.
+    - intro H. exists (ofun_app x celem); [ assumption | reflexivity ]. }
+  { intro x; simpl; split.
+    - intros [ z pf1 pf2 ]. rewrite <- flipLeftAdj in pf1.
+      rewrite <- pf1. assumption.
+    - intro. exists (unflip x); [ reflexivity | ]. destruct x; assumption. }
+  { intro c; simpl; split.
+    - intros [ b pf_bc [ a pf_ab pf_a ] ].
+      exists a; [ exists b | ]; assumption.
+    - intros [ a [ b pf_bc pf_ab ] pf_a ].
+      exists b; [ | exists a ]; assumption. }
+Qed.
+
+
+Instance MonadBottomOps_DownSet : MonadBottomOps DownSet :=
+  {| bottomM := fun _ _ => oexpr (ofun b => oFalse) |}.
+
+Instance MonadBottom_DownSet : MonadBottom DownSet.
+Proof.
+  constructor; [ typeclasses eauto | ].
+  intros. intros a1 a2 Ra a3 a4 R34 pf_false. destruct pf_false.
+Qed.
+
+
+Definition fixDownSet {A B} `{OType A} `{OType B} :
+  ((A -o> DownSet B) -o> (A -o> DownSet B)) -o> A -o> DownSet B :=
+  oexpr
+    (ofun f => ofun a => ofun b =>
+     oforall @o@ (ofun g =>
+                  oimpl @o@ (oflip (oappr
+                                      @o@ oflip' (ovar f @o@ ounequiv (ovar g))
+                                      @o@ ounequiv' (ovar g)))
+                        @o@ (ounequiv (ovar g) @o@ ovar a @o@ ovar b)
+    )).
+
+Instance MonadFixOps_DownSet : MonadFixOps DownSet := {| fixM := @fixDownSet |}.
+
+Instance MonadFix_DownSet : MonadFix DownSet.
+Admitted.
