theories/OExpr.v
@@ -1,0 +1,548 @@
+Require Export SepTypes.OrderedType.
+Require Export SepTypes.OFuns.
+
+
+(***
+ *** Ordered Type Contexts
+ ***)
+
+(* A context here is just a list of type expressions *)
+Inductive Ctx : Type :=
+| CNil
+| CCons (ctx:Ctx) A {RA:OType A}
+.
+
+Notation "ctx :> A" := (CCons ctx A) (left associativity, at level 50).
+
+(* An element of a context is a nested tuple of elements of its types *)
+Fixpoint CtxElem (ctx:Ctx) : Type :=
+  match ctx with
+  | CNil => unit
+  | ctx' :> A => CtxElem ctx' * A
+  end.
+
+(* OTRelation instance for any CtxElem type *)
+Instance OType_CtxElem ctx : OType (CtxElem ctx).
+Proof.
+  induction ctx; typeclasses eauto.
+Defined.
+
+(* Typeclasses Transparent OType_CtxElem. *)
+
+Definition ctxHead ctx : Type :=
+  match ctx with
+  | CNil => unit
+  | CCons _ A => A
+  end.
+
+Instance OType_ctxHead ctx : OType (ctxHead ctx) :=
+  match ctx with
+  | CNil => OTunit
+  | @CCons _ _ RA => RA
+  end.
+
+Definition ctxTail ctx :=
+  match ctx with
+  | CNil => CNil
+  | ctx' :> _ => ctx'
+  end.
+
+
+(***
+ *** Ordered Expressions and Variables
+ ***)
+
+(* An ordered expression in ctx is just a Proper function from ctx *)
+Definition OExpr ctx A `{OType A} : Type := CtxElem ctx -o> A.
+
+Arguments OExpr ctx A {_} : simpl never.
+
+(* Low-level lambda (we use "ofun", below, to give a nice high-level lambda) *)
+(* Notation "'olambda' e" := (ofun_curry e) (at level 99, right associativity). *)
+
+Inductive OVar : Ctx -> forall A `{OType A}, Type :=
+| OVar_0 {ctx A} `{OType A} : OVar (ctx :> A) A
+| OVar_S {ctx B A} `{OType A} `{OType B} (v: OVar ctx A) : OVar (ctx :> B) A
+.
+
+(* The last-bound variable in a context *)
+Definition var_top {ctx A} `{OType A} : OExpr (ctx :> A) A :=
+  {| ofun_app := snd; ofun_Proper := _ |}.
+
+(* Weaken an OExpr by adding a type to the context *)
+Definition weaken1 {ctx A B} `{OType A} `{OType B}
+           (e: OExpr ctx A) : OExpr (ctx :> B) A :=
+  compose_ofun fst_ofun e.
+
+Fixpoint varSemantics {ctx A} `{OType A} (v:OVar ctx A) : OExpr ctx A :=
+  match v in OVar ctx' A' return OExpr ctx' A' with
+  | OVar_0 => var_top
+  | OVar_S v => weaken1 (varSemantics v)
+  end.
+
+Coercion varSemantics : OVar >-> OExpr.
+
+
+(***
+ *** Weakening
+ ***)
+
+(* Inductive proof that ctx1 can be weakened to ctx2 *)
+Inductive weakensTo ctx1 : Ctx -> Type :=
+| WeakensRefl : weakensTo ctx1 ctx1
+| WeakensCons {ctx2} (w: weakensTo ctx1 ctx2) A `{OType A}  :
+    weakensTo ctx1 (ctx2 :> A)
+.
+
+Arguments WeakensRefl {_}.
+Arguments WeakensCons {_ _} w A {_}.
+
+(* Typeclass version of the above *)
+Class WeakensTo ctx1 ctx2 : Type :=
+  weakensProof : weakensTo ctx1 ctx2.
+
+Instance WeakensTo_refl ctx : WeakensTo ctx ctx := WeakensRefl.
+
+Instance WeakensTo_cons ctx1 ctx2 A `{OType A} (w: WeakensTo ctx1 ctx2) :
+  WeakensTo ctx1 (ctx2 :> A) :=
+  WeakensCons w A.
+
+(* Weaken a context by mapping backwardds from the weaker to the stronger one *)
+Fixpoint weakenContext {ctx1 ctx2} (w: weakensTo ctx1 ctx2) :
+  CtxElem ctx2 -o> CtxElem ctx1 :=
+  match w in weakensTo _ ctx2 return CtxElem ctx2 -o> CtxElem ctx1 with
+  | WeakensRefl => id_ofun
+  | WeakensCons w' _ => compose_ofun fst_ofun (weakenContext w')
+  end.
+
+(* Weakening for OExprs *)
+Definition weakenExpr {ctx1 ctx2} `{w: WeakensTo ctx1 ctx2} {A} `{OType A}
+           (e: OExpr ctx1 A) : OExpr ctx2 A :=
+  compose_ofun (weakenContext w) e.
+
+Instance Proper_weakenExpr {ctx1 ctx2} `{w: WeakensTo ctx1 ctx2} {A} `{OType A} :
+  Proper (oleq ==> oleq) (weakenExpr (w:=w) (A:=A)).
+Proof.
+  intros e1 e2 Re. apply Proper_compose_ofun; [ reflexivity | assumption ].
+Qed.
+
+(* Weakening for variables *)
+Fixpoint weakenVar_h {ctx1 ctx2} (w: weakensTo ctx1 ctx2) :
+  forall {A} `{OType A}, OVar ctx1 A -> OVar ctx2 A :=
+  match w in weakensTo _ ctx2
+        return forall {A} `{OType A}, OVar ctx1 A -> OVar ctx2 A
+  with
+  | WeakensRefl => fun _ _ v => v
+  | WeakensCons w' _ => fun _ _ v => OVar_S (weakenVar_h w' v)
+  end.
+
+Definition weakenVar {ctx1 ctx2} `{w:WeakensTo ctx1 ctx2} {A} `{OType A}
+           (v:OVar ctx1 A) : OVar ctx2 A :=
+  weakenVar_h w v.
+
+(* Weakening is the same whether we do it before or after varSemantics *)
+Lemma weakenVar_weakenExpr {ctx1 ctx2} `{w:WeakensTo ctx1 ctx2} {A} `{OType A}
+      (v:OVar ctx1 A) : weakenExpr (w:=w) v =o= weakenVar v.
+Proof.
+  revert v; induction w; intro v; simpl.
+  { apply id_compose_ofun. }
+  { unfold weaken1. rewrite <- IHw. unfold weakenExpr. simpl.
+    rewrite compose_compose_ofun. reflexivity. }
+Qed.
+
+
+(***
+ *** Substitution
+ ***)
+
+(* A substitution for a single variable in a ctx *)
+Fixpoint CtxSubst ctx : Type :=
+  match ctx with
+  | CNil => False
+  | ctx' :> A => CtxSubst ctx' + OExpr ctx' A
+  end.
+
+(* The output context of a substitution *)
+Fixpoint CtxSubstCtx {ctx} : CtxSubst ctx -> Ctx :=
+  match ctx return CtxSubst ctx -> Ctx with
+  | CNil => fun empty => match empty with end
+  | ctx' :> A => fun subst_or_expr =>
+                   match subst_or_expr with
+                   | inl subst' => CtxSubstCtx subst' :> A
+                   | inr _ => ctx'
+                   end
+  end.
+
+(* The output type of a substitution *)
+Fixpoint CtxSubstType {ctx} : CtxSubst ctx -> Type :=
+  match ctx return CtxSubst ctx -> Type with
+  | CNil => fun empty => match empty with end
+  | ctx' :> A => fun subst_or_expr =>
+                   match subst_or_expr with
+                   | inl subst' => CtxSubstType subst'
+                   | inr _ => A
+                   end
+  end.
+
+Fixpoint CtxSubstOType {ctx} : forall s, OType (@CtxSubstType ctx s) :=
+  match ctx return forall s, OType (@CtxSubstType ctx s) with
+  | CNil => fun empty => match empty with end
+  | ctx' :> A => fun subst_or_expr =>
+                   match subst_or_expr with
+                   | inl subst' => CtxSubstOType subst'
+                   | inr _ => _
+                   end
+  end.
+
+Instance OType_CtxSubstType ctx s : OType (@CtxSubstType ctx s) :=
+  CtxSubstOType s.
+
+(* Use a substitution like a mapping *)
+Fixpoint substContext {ctx} :
+  forall (s: CtxSubst ctx), CtxElem (CtxSubstCtx s) -o> CtxElem ctx :=
+  match ctx return forall (s: CtxSubst ctx), CtxElem (CtxSubstCtx s) -o>
+                                             CtxElem ctx
+  with
+  | CNil => fun empty => match empty with end
+  | ctx' :> A =>
+    fun s =>
+      match s return CtxElem (@CtxSubstCtx (_ :> _) s) -o> CtxElem (_ :> _) with
+      | inl s' => pair_ofun (compose_ofun fst_ofun (substContext s')) snd_ofun
+      | inr e => pair_ofun id_ofun e
+      end
+  end.
+
+Definition substExpr {ctx A} `{OType A} (e: OExpr ctx A) (s: CtxSubst ctx) :
+  OExpr (CtxSubstCtx s) A :=
+  compose_ofun (substContext s) e.
+
+(* The result of looking up a variable in a substitution; see substVarLookup *)
+Inductive VarLookupRes ctx A `{OType A} (s:CtxSubst ctx) : Type :=
+| mkVarLookupRes ctx' (w: weakensTo ctx' (CtxSubstCtx s))
+                 (v_or_e: OVar ctx' A + OExpr ctx' A) :
+    VarLookupRes ctx A s.
+
+(* Weaken a VarLookupRes *)
+Definition weakenVarLookupRes {ctx A B} `{OType A} `{OType B} {s}
+           (res: VarLookupRes ctx A s) :
+  VarLookupRes (ctx :> B) A (inl s) :=
+  match res with
+  | mkVarLookupRes _ _ _ ctx' w v_or_e =>
+    mkVarLookupRes (_:>_) A (inl s) ctx' (WeakensCons w B) v_or_e
+  end.
+
+(* Look up a variable in a substitution, getting either an OExpr or a
+strengthened variable. We existentially quantify over the returned context so
+that we can do one combined weakening, either of the returned variable or oexpr,
+rather than having N weakening steps *)
+Program Fixpoint substVarLookup {ctx A} `{OType A} (v: OVar ctx A) :
+  forall (s:CtxSubst ctx), VarLookupRes ctx A s :=
+  match v in OVar ctx A return forall s, VarLookupRes ctx A s with
+  | OVar_0 =>
+    fun (s: CtxSubst (_ :> _)) =>
+      match s return VarLookupRes (_:>_) _ s
+      with
+      | inl s' =>
+        mkVarLookupRes (_:>_) _ (inl s') _ WeakensRefl (inl OVar_0)
+      | inr e =>
+        mkVarLookupRes (_:>_) _ (inr e) _ WeakensRefl (inr e)
+      end
+  | OVar_S v' =>
+    fun (s: CtxSubst (_:>_)) =>
+      match s return VarLookupRes (_:>_) _ s with
+      | inl s' =>
+        weakenVarLookupRes (substVarLookup v' s')
+      | inr e =>
+        mkVarLookupRes (_:>_) _ (inr e) _ WeakensRefl (inl v')
+      end
+  end.
+
+(* Substitute into a variable *)
+Definition substVar {ctx A} `{OType A} (v: OVar ctx A) (s:CtxSubst ctx) :
+  OExpr (CtxSubstCtx s) A :=
+  match substVarLookup v s with
+  | mkVarLookupRes _ _ _ ctx' w (inl v') => weakenVar_h w v'
+  | mkVarLookupRes _ _ _ ctx' w (inr e) => weakenExpr (w:=w) e
+  end.
+
+(* Substitution is the same whether we do it before or after varSemantics *)
+Lemma substVar_substExpr {ctx} {A} `{OType A} (v: OVar ctx A)
+      (s: CtxSubst ctx) : substExpr v s =o= substVar v s.
+Proof.
+  revert s; induction v; intro s; unfold substExpr.
+  { destruct s as [ s | e ]; simpl; apply funOExt; intro c; reflexivity. }
+  { destruct s as [ s | e ]; simpl; apply funOExt; intro c; [ | reflexivity ].
+    simpl.
+    assert ((substVar (OVar_S v) (inl s)) = weakenExpr (substVar v s)).
+    - unfold substVar. simpl. destruct (substVarLookup v s); simpl.
+      destruct v_or_e; admit.
+    - rewrite H1. rewrite <- IHv. reflexivity. }
+Admitted.
+
+
+(***
+ *** Notation for Application
+ ***)
+
+(* FIXME: weaken both sides to a join of their respective contexts! *)
+Definition oexpr_apply {ctx A B} `{OType A} `{OType B}
+           (f: OExpr ctx (A -o> B)) (g: OExpr ctx A) : OExpr ctx B :=
+  ofun_apply f g.
+
+(* Application *)
+Notation "x @o@ y" :=
+  (oexpr_apply x y) (left associativity, at level 20).
+
+
+(***
+ *** Notation for Variables, Lambdas, and Top-level Expressions
+ ***)
+
+Definition oexpr {A} `{OType A} (e: OExpr CNil A) : A := ofun_app e tt.
+
+Definition ovar {ctx A} `{OType A} {ctx'} `{w:WeakensTo ctx ctx'}
+           (e:OExpr ctx A) : OExpr ctx' A := weakenExpr e.
+
+(* Helper function to build lambdas *)
+(*
+Definition mkLam {ctx A B} `{OType A} `{OType B}
+           (body : (forall {ctx'} `{WeakensTo (ctx :> A) ctx'}, OVar ctx' A) ->
+                   OExpr (ctx :> A) B) :
+  OExpr ctx (A -o> B) :=
+  ofun_curry (body (fun _ _ => weakenVar OVar_0)).
+ *)
+
+Definition mkLam {ctx A B} `{OType A} `{OType B}
+           (body : OVar (ctx :> A) A -> OExpr (ctx :> A) B) :
+  OExpr ctx (A -o> B) := ofun_curry (body OVar_0).
+
+Notation "'ofun' x => e" :=
+  (mkLam (fun x => e))
+    (right associativity, at level 99).
+
+Notation "'ofun' ( x : A ) => e" :=
+  (mkLam (fun (x : OVar _ A) => e))
+    (right associativity, at level 99, x at level 0).
+
+
+(***
+ *** Ordered Expressions for Unit
+ ***)
+
+Definition ott {ctx} : OExpr ctx unit := const_ofun tt.
+
+Lemma ott_terminal {ctx} (e: OExpr ctx unit) : e =o= ott.
+Proof.
+  apply funOExt; intro c. destruct (e @@ c). reflexivity.
+Qed.
+
+
+(***
+ *** Ordered Expressions for Pairs
+ ***)
+
+Definition opair {ctx A B} `{OType A} `{OType B} : OExpr ctx (A -o> B -o> A*B) :=
+  const_ofun (ofun_curry id_ofun).
+Definition ofst {ctx A B} `{OType A} `{OType B} : OExpr ctx (A * B -o> A) :=
+  const_ofun fst_ofun.
+Definition osnd {ctx A B} `{OType A} `{OType B} : OExpr ctx (A * B -o> B) :=
+  const_ofun snd_ofun.
+
+Notation "( x ,o, y )" := (opair @o@ x @o@ y : OExpr _ _) (at level 0).
+
+Lemma ofst_opair {ctx A B} `{OType A} `{OType B}
+      (e1: OExpr ctx A) (e2: OExpr ctx B) :
+  ofst @o@ (e1 ,o, e2) =o= e1.
+Proof.
+  apply funOExt; intro c. reflexivity.
+Qed.
+
+Lemma osnd_opair {ctx A B} `{OType A} `{OType B}
+      (e1: OExpr ctx A) (e2: OExpr ctx B) :
+  osnd @o@ (e1 ,o, e2) =o= e2.
+Proof.
+  apply funOExt; intro c. reflexivity.
+Qed.
+
+Lemma opair_ext {ctx A B} `{OType A} `{OType B} (e: OExpr ctx (A*B)) :
+  opair @o@ (ofst @o@ e) @o@ (osnd @o@ e) =o= e.
+Proof.
+  apply funOExt; intro c. simpl. destruct (ofun_app e c). reflexivity.
+Qed.
+
+
+(***
+ *** Ordered Expressions for Sums
+ ***)
+
+Definition oinl {ctx A B} `{OType A} `{OType B} : OExpr ctx (A -o> A + B) :=
+  const_ofun inl_ofun.
+Definition oinr {ctx A B} `{OType A} `{OType B} : OExpr ctx (B -o> A + B) :=
+  const_ofun inr_ofun.
+Definition osumElim {ctx A B C} `{OType A} `{OType B} `{OType C} :
+  OExpr ctx ((A -o> C) -o> (B -o> C) -o> A + B -o> C) :=
+  const_ofun sum_elim_ofun.
+
+Lemma osumElim_oinl {ctx A B C} `{OType A} `{OType B} `{OType C}
+      (f1 : OExpr ctx (A -o> C)) (f2 : OExpr ctx (B -o> C)) e :
+  osumElim @o@ f1 @o@ f2 @o@ (oinl @o@ e) =o= f1 @o@ e.
+Proof.
+  apply funOExt; intro c. reflexivity.
+Qed.
+
+Lemma osumElim_oinr {ctx A B C} `{OType A} `{OType B} `{OType C}
+      (f1 : OExpr ctx (A -o> C)) (f2 : OExpr ctx (B -o> C)) e :
+  osumElim @o@ f1 @o@ f2 @o@ (oinr @o@ e) =o= f2 @o@ e.
+Proof.
+  apply funOExt; intro c. reflexivity.
+Qed.
+
+
+(***
+ *** Ordered Expressions for Propositions
+ ***)
+
+Definition oTrue {ctx} : OExpr ctx Prop := const_ofun True.
+Definition oFalse {ctx} : OExpr ctx Prop := const_ofun False.
+
+Definition oforall {ctx A} `{OType A} : OExpr ctx ((A -o> Prop) -o> Prop) :=
+  const_ofun forall_ofun.
+Definition oexists {ctx A} `{OType A} : OExpr ctx ((A -o> Prop) -o> Prop) :=
+  const_ofun exists_ofun.
+Definition oexists2 {ctx A} `{OType A} :
+  OExpr ctx ((A -o> Prop) -o> (Flip A -o> Prop) -o> Prop) :=
+  const_ofun exists2flip_ofun.
+
+Definition oand {ctx} : OExpr ctx (Prop -o> Prop -o> Prop) :=
+  const_ofun and_ofun.
+Definition oor {ctx} : OExpr ctx (Prop -o> Prop -o> Prop) :=
+  const_ofun or_ofun.
+Definition oimpl {ctx} : OExpr ctx (Flip Prop -o> Prop -o> Prop) :=
+  const_ofun impl_ofun.
+Definition oappr {ctx A} `{OType A} : OExpr ctx (Flip A -o> A -o> Prop) :=
+  const_ofun oleq_ofun.
+
+
+(***
+ *** Flip and Equiv Types
+ ***)
+
+Fixpoint flipCtx (ctx : Ctx) :=
+  match ctx with
+  | CNil => CNil
+  | ctx' :> A => flipCtx ctx' :> Flip A
+  end.
+
+Fixpoint flipCtxElem {ctx} : CtxElem ctx -> CtxElem (flipCtx ctx) :=
+  match ctx return CtxElem ctx -> CtxElem (flipCtx ctx) with
+  | CNil => fun celem => celem
+  | ctx' :> A => fun celem => (flipCtxElem (fst celem), flip (snd celem))
+  end.
+
+Instance Proper_flipCtxElem ctx : Proper (oleq --> oleq) (@flipCtxElem ctx).
+Proof.
+  induction ctx; intros c1 c2 Rc.
+  - destruct c1; destruct c2; reflexivity.
+  - destruct Rc. split; [ apply IHctx | ]; assumption.
+Qed.
+
+Fixpoint unflipCtxElem {ctx} : CtxElem (flipCtx ctx) -> CtxElem ctx :=
+  match ctx return CtxElem (flipCtx ctx) -> CtxElem ctx with
+  | CNil => fun celem => celem
+  | ctx' :> A => fun celem => (unflipCtxElem (fst celem), unflip (snd celem))
+  end.
+
+Instance Proper_unflipCtxElem ctx : Proper (oleq --> oleq) (@unflipCtxElem ctx).
+Proof.
+  induction ctx; intros c1 c2 Rc.
+  - destruct c1; destruct c2; reflexivity.
+  - destruct Rc. split; [ apply IHctx | ]; assumption.
+Qed.
+
+Lemma flipCtxElem_unflipCtxElem ctx (celem: CtxElem ctx) :
+  unflipCtxElem (flipCtxElem celem) =o= celem.
+Proof.
+  revert celem; induction ctx; intros; [ reflexivity | ].
+  destruct celem. destruct (IHctx c).
+  split; split; try reflexivity; assumption.
+Qed.
+
+Lemma unflipCtxElem_flipCtxElem ctx (celem: CtxElem (flipCtx ctx)) :
+  flipCtxElem (unflipCtxElem celem) =o= celem.
+Proof.
+  revert celem; induction ctx; intros; [ reflexivity | ].
+  destruct celem. destruct (IHctx c). simpl. rewrite flip_unflip.
+  split; split; try reflexivity; assumption.
+Qed.
+
+
+(* A "flipped" ordered expression *)
+Definition OExprFlip ctx A `{OType A} : Type := OExpr (flipCtx ctx) A.
+
+Arguments OExprFlip ctx A {_} : simpl never.
+
+Program Definition oflip {ctx A} `{OType A} (e: OExprFlip ctx A)
+  : OExpr ctx (Flip A) :=
+  {| ofun_app := fun celem => flip (e @@ flipCtxElem celem) |}.
+Next Obligation.
+  intros c1 c2 Rc. simpl. rewrite Rc. reflexivity.
+Defined.
+
+Program Definition ounflip {ctx A} `{OType A} (e: OExpr ctx (Flip A))
+  : OExprFlip ctx A :=
+  {| ofun_app := fun celem => unflip (e @@ unflipCtxElem celem) |}.
+Next Obligation.
+  intros c1 c2 Rc. simpl. rewrite Rc. reflexivity.
+Defined.
+
+Lemma oflip_ounflip {ctx A} `{OType A} (e: OExprFlip ctx A) :
+  ounflip (oflip e) =o= e.
+  revert e; induction ctx; intros; apply funOExt; intro c; [ reflexivity | ].
+  simpl. rewrite flip_unflip. rewrite unflipCtxElem_flipCtxElem.
+  destruct c; reflexivity.
+Qed.
+
+Lemma ounflip_oflip {ctx A} `{OType A} (e: OExpr ctx (Flip A)) :
+  oflip (ounflip e) =o= e.
+  revert e; induction ctx; intros; apply funOExt; intros c; simpl;
+    rewrite flip_unflip; [ reflexivity | ].
+  rewrite flipCtxElem_unflipCtxElem. destruct c; reflexivity.
+Qed.
+
+Program Definition oflip' {ctx A} `{OType A} (e: OExpr ctx A)
+  : OExprFlip ctx (Flip A) :=
+  {| ofun_app := fun celem => flip (e @@ unflipCtxElem celem) |}.
+Next Obligation.
+  intros c1 c2 Rc. simpl. rewrite Rc. reflexivity.
+Defined.
+
+Program Definition ounflip' {ctx A} `{OType A} (e: OExprFlip ctx (Flip A))
+  : OExpr ctx A :=
+  {| ofun_app := fun celem => unflip (e @@ flipCtxElem celem) |}.
+Next Obligation.
+  intros c1 c2 Rc. simpl. rewrite Rc. reflexivity.
+Defined.
+
+Lemma oflip'_ounflip' {ctx A} `{OType A} (e: OExpr ctx A) :
+  ounflip' (oflip' e) =o= e.
+  revert e; induction ctx; intros; apply funOExt; intro c; [ reflexivity | ].
+  simpl. rewrite flipCtxElem_unflipCtxElem.
+  destruct c; reflexivity.
+Qed.
+
+Lemma ounflip'_oflip' {ctx A} `{OType A} (e: OExprFlip ctx (Flip A)) :
+  oflip' (ounflip' e) =o= e.
+  revert e; induction ctx; intros; apply funOExt; intros c; simpl;
+    rewrite flip_unflip; [ reflexivity | ].
+  rewrite unflipCtxElem_flipCtxElem. rewrite flip_unflip.
+  destruct c; reflexivity.
+Qed.
+
+
+Definition ounequiv {ctx A} `{OType A} (e : OExpr ctx (Equiv A)) :
+  OExpr ctx A :=
+  compose_ofun e unequiv_ofun.
+
+Program Definition ounequiv' {ctx A} `{OType A} (e : OExpr ctx (Equiv A)) :
+  OExprFlip ctx A :=
+  ounflip (compose_ofun e unequiv'_ofun).
